src/tlogic/LogicSyntaxHOAS.v
@@ -19,10 +19,10 @@ Module Syntax.
     (* | prodT : type -> type -> type *)
     (* | sumT : type -> type -> type *)
     (* | listT : type -> type *)
-    (* | funT : type -> type -> type *)
+    | funT : type -> type -> type.
     (* | positiveT : type *)
-    | pgmapT : type -> type.
-    (* | gmapTpos : type -> type. *)
+    (* | pgmapT : type -> type *)
+    (* | gmapTpos : type -> typ. *)
     (* | gmapT (K : Type) {EqDec : EqDecision K} {Cnt : Countable K} : type -> type. *)
 
   (* If we define for a general gmapT with EqDec and Countable,
@@ -93,9 +93,9 @@ Module Syntax.
       (* | prodT ty1 ty2 => prod (Typ_0 ty1) (Typ_0 ty2) *)
       (* | sumT ty1 ty2 => sum (Typ_0 ty1) (Typ_0 ty2) *)
       (* | listT ty' => list (Typ_0 ty') *)
-      (* | funT ty1 ty2 => (Typ_0 ty1 -> Typ_0 ty2) *)
+      | funT ty1 ty2 => (Typ_0 form ty1 -> Typ_0 form ty2)
       (* | positiveT => positive *)
-      | pgmapT ty' => gmap positive (Typ_0 form ty')
+      (* | pgmapT ty' => gmap positive (Typ_0 form ty') *)
       (* | gmapTpos ty' => gmap positive (Typ_0 ty') *)
       (* | @gmapT _ K EqDec Cnt ty' => @gmap K EqDec Cnt (Typ_0 ty') *)
       end.
@@ -174,7 +174,7 @@ Module Syntax.
       | upd p => Upd (to_semantics_0 n sem p)
       end.
 
-    Definition cast_typing n : typing (S n) formulaT -> @t (typing n) (As (typing n)) :=
+    Let cast_typing n : typing (S n) formulaT -> @t (typing n) (As (typing n)) :=
       fun p => p.
 
     Fixpoint to_semantics n : @t (typing n) (As (typing n)) -> iProp :=
@@ -354,55 +354,40 @@ Module Syntax.
 
   End RED.
 
-  Section GMAP.
+  (* Section GMAP. *)
 
-    Context `{Σ : GRA.t}.
-    (* Context `{T : Type}. *)
-    (* Context `{TSem : T -> Type}. *)
-    Context `{As : (type -> Type) -> Type}.
-    (* Context `{As : (@type T -> Type) -> Type}. *)
+  (*   Context `{Σ : GRA.t}. *)
+  (*   Context `{As : (type -> Type) -> Type}. *)
 
-    Local Notation typing := (@Typ As).
-    Local Notation Formulas := (fun (i : index) => @t (typing i) (As (typing i))).
-    (* Local Notation typing := (@Typ T TSem As). *)
-    (* Local Notation Formulas := (fun (i : index) => @t T (typing i) (As (typing i))). *)
+  (*   Local Notation typing := (@Typ As). *)
+  (*   Local Notation Formulas := (fun (i : index) => @t (typing i) (As (typing i))). *)
 
-    Context `{interp_atoms : forall (n : index), As (typing n) -> iProp}.
+  (*   Context `{interp_atoms : forall (n : index), As (typing n) -> iProp}. *)
 
-    (* Maybe we can make Syntax as an instance of bi. *)
-    Definition star_gmap
-               (n : index) (I : typing (S n) (pgmapT formulaT))
-               (f : positive -> Formulas n -> Formulas n)
-      : Formulas n :=
-      fold_right (fun hd tl => @sepconj (typing n) (As (typing n)) (uncurry f hd) tl) empty (map_to_list I).
+  (*   (* Maybe we can make Syntax as an instance of bi. *) *)
+  (*   Definition star_gmap *)
+  (*              (n : index) (I : typing (S n) (pgmapT formulaT)) *)
+  (*              (f : positive -> Formulas n -> Formulas n) *)
+  (*     : Formulas n := *)
+  (*     fold_right (fun hd tl => @sepconj (typing n) (As (typing n)) (uncurry f hd) tl) empty (map_to_list I). *)
 
-    (* Definition star_gmap (n : index) (I : typing (S n) (gmapTpos formulaT)) (f : typing (S n) (funT positiveT (funT formulaT formulaT))) *)
-    (*   : Formulas n. *)
-    (* Proof. *)
-    (*   ss. *)
-    (*   refine *)
-    (*     (fold_right (fun hd tl => @sepconj T (typing n) (As (typing n)) (uncurry f hd) tl) empty (map_to_list I)). *)
-    (* Defined. *)
 
-    Local Notation Sem := (fun i p => @to_semantics Σ As interp_atoms i p).
-    (* Local Notation Sem := (fun i p => @to_semantics Σ T TSem As interp_atoms i p). *)
+  (*   Local Notation Sem := (fun i p => @to_semantics Σ As interp_atoms i p). *)
 
-    Lemma star_gmap_iProp
-          n I f
-      :
-      Sem n (star_gmap n I f) =
-        ([∗ map] i ↦ p ∈ I, Sem n (f i p))%I.
-    Proof.
-      ss. unfold big_opM. rewrite seal_eq. unfold big_op.big_opM_def.
-      unfold star_gmap. ss. remember (map_to_list I) as L.
-      (* etransitivity. instantiate (1:= ([∗ list] x ∈ L, uncurry (λ (i : positive) (p : t), to_semantics n (f i p)) x)%I). *)
-      (* 2:{ subst. reflexivity. } *)
-      clear HeqL I. induction L.
-      { ss. apply to_semantics_empty. }
-      ss. rewrite to_semantics_red_sepconj. rewrite IHL. f_equal.
-      destruct a. ss.
-    Qed.
+  (*   Lemma star_gmap_iProp *)
+  (*         n I f *)
+  (*     : *)
+  (*     Sem n (star_gmap n I f) = *)
+  (*       ([∗ map] i ↦ p ∈ I, Sem n (f i p))%I. *)
+  (*   Proof. *)
+  (*     ss. unfold big_opM. rewrite seal_eq. unfold big_op.big_opM_def. *)
+  (*     unfold star_gmap. ss. remember (map_to_list I) as L. *)
+  (*     clear HeqL I. induction L. *)
+  (*     { ss. apply to_semantics_empty. } *)
+  (*     ss. rewrite to_semantics_red_sepconj. rewrite IHL. f_equal. *)
+  (*     destruct a. ss. *)
+  (*   Qed. *)
 
-  End GMAP.
+  (* End GMAP. *)
 
 End Syntax.
