src/tlogic/TemporalLogic.v
@@ -9,6 +9,8 @@ From iris Require base_logic.lib.invariants.
 
 Local Notation index := nat.
 
+TODO
+
 Section Atom.
 
   Context `{Σ : GRA.t}.
